sample_mark/verif_unionfind.v
@@ -50,7 +50,7 @@ Definition find_spec :=
           SEP   (graph sh x g)
   POST [ tptr (Tstruct _Node noattr) ]
         EX g': Graph, EX rt : pointer_val,
-        PROP (uf_equiv g g' /\ uf_root g' x rt /\ rank_unchanged g g')
+        PROP (findS g x g' /\ uf_root g' x rt)
         LOCAL (temp ret_temp (pointer_val_val rt))
         SEP (vertices_at sh (reachable g x) g').
 
@@ -115,14 +115,17 @@ Proof.
     (@data_at CompSpecs sh node_type (Vint (Int.repr 0), pointer_val_val x)).
     apply (exp_right (single_Graph x x_not_null O tt tt)). entailer.
     apply (exp_right x). entailer !.
-    + simpl. apply single_uf_is_uf.
+    + simpl. apply single_uf_is_uf. auto.
     + unfold reachable_vertices_at. simpl. unfold vertices_at. unfold iter_sepcon.pred_sepcon.
       apply (exp_right (x:: nil)). entailer !.
       * simpl. split.
-        -- intros. rewrite reachabel_single_uf. intuition.
+        -- intros. rewrite reachabel_single_uf. intuition. auto.
         -- constructor. intuition. constructor.
       * simpl. unfold graph_vcell. unfold vgamma. simpl. unfold graph_gen.updateEdgeFunc.
-        destruct (EquivDec.equiv_dec (x, tt) (x, tt)); entailer !.
+        assert ((if EquivDec.equiv_dec (x, tt) (x, tt) then null else x) = null) by (destruct (EquivDec.equiv_dec (x, tt) (x, tt)); [|compute in c; exfalso]; auto).
+        rewrite H2. assert ((if SGBA_VE null null then x else null) = x). {
+          Transparent pSGG_VST. compute. Opaque pSGG_VST. destruct (PV_eq_dec NullPointer NullPointer); [|exfalso]; auto.
+        } rewrite H3. entailer !.
 Qed.
 
 Lemma body_find: semax_body Vprog Gprog f_find find_spec.
@@ -151,13 +154,13 @@ Proof.
   unfold semax_ram.
   forward_if_tac
     (EX g': Graph, EX rt : pointer_val,
-     PROP (uf_equiv g g' /\ uf_root g' x rt /\ rank_unchanged g g')
-     LOCAL (temp _p (pointer_val_val rt))
+     PROP (findS g x g' /\ uf_root g' x rt)
+     LOCAL (temp _p (pointer_val_val rt); temp _x (pointer_val_val x))
      SEP (vertices_at sh (reachable g x) g'));
     [apply ADMIT | | gather_current_goal_with_evar ..].
   localize
     (PROP (vvalid g pa)
-     LOCAL (temp _p (pointer_val_val pa))
+     LOCAL (temp _p (pointer_val_val pa); temp _x (pointer_val_val x))
      SEP (graph sh pa g)).
   1: symmetry in H0; apply valid_parent in H0; auto.
   eapply semax_ram_seq;
@@ -168,7 +171,8 @@ Proof.
       apply ram_extract_PROP; intros]. destruct H3 as [? [? ?]].
     unlocalize
       (PROP ()
-       LOCAL (temp _p0 (pointer_val_val x'); temp _p (pointer_val_val pa))
+       LOCAL (temp _p0 (pointer_val_val x'); temp _p (pointer_val_val pa);
+              temp _x (pointer_val_val x))
        SEP (vertices_at sh (reachable g x) g'))
     using [H3; H4; H5]%RamAssu
     binding [g'; x']%RamBind.
@@ -186,13 +190,57 @@ Proof.
         + symmetry in Heqb1. apply binop_lemmas2.int_eq_true in Heqb1. subst; auto.
         + simpl in H1. inversion H1.
       - simpl in H1. inversion H1.
-    } subst pa. split; [|split; [split |]]; auto.
+    } subst pa. split; split; [|split| |]; auto.
+    - reflexivity.
     - apply (uf_equiv_refl _  (liGraph g)).
-    - apply uf_root_vgamma with (n := r); auto.
     - repeat intro; auto.
+    - apply uf_root_vgamma with (n := r); auto.
   } Unfocus.
   Focus 2. {
-    simplify_ramif. 
+    simplify_ramif. apply (@graph_ramify_aux_parent _ (sSGG_VST sh) _ g x r); auto.
+  } Unfocus.
+  unfold semax_ram.
+  forward.
+  assert (pa <> x). {
+    hnf in H1. destruct pa, x; inversion H1; [|intro; inversion H6..].
+    simpl in H1. clear H7. unfold sem_cmp_pp in H1.
+    simpl in H1. destruct (eq_block b b0).
+    - destruct (Int.eq i i0) eqn:? .
+      + simpl in H1. inversion H1.
+      + subst b0. apply int_eq_false_e in Heqb1. intro. inversion H6. auto.
+    - intro. inversion H6. auto.
+  } assert (weak_valid g' x') by (right; apply reachable_foot_valid in H4; auto).
+  assert (vvalid g' x) by (destruct H3 as [_ [[? _] _]]; rewrite <- H3; apply H).
+  assert ((vgamma g' x) = (r, pa)) by (apply (findS_preserves_vgamma g); auto).
+  assert (~ reachable g' x' x) by (apply (vgamma_not_reachable' _ _ r pa); auto).
+  localize
+   (PROP  ()
+    LOCAL (temp _p (pointer_val_val x'); temp _x (pointer_val_val x))
+    SEP   (data_at sh node_type (Vint (Int.repr (Z.of_nat r)), pointer_val_val pa)
+                   (pointer_val_val x))).
+    eapply semax_ram_seq';
+    [ subst RamFrame RamFrame0; unfold abbreviate;
+      repeat apply eexists_add_stats_cons; constructor
+    | store_tac 
+    | abbreviate_semax_ram].
+    assert (force_val (sem_cast_neutral (pointer_val_val x')) = pointer_val_val x'). {
+      destruct x'; simpl; auto.
+    } rewrite H11. clear H11.
+    change (@field_at CompSpecs sh node_type [] (Vint (Int.repr (Z.of_nat r)), pointer_val_val x') (pointer_val_val x)) with
+    (@data_at CompSpecs sh node_type (Vint (Int.repr (Z.of_nat r)), pointer_val_val x') (pointer_val_val x)).
+    unlocalize
+      (PROP ()
+       LOCAL (temp _p (pointer_val_val x'); temp _x (pointer_val_val x))
+       SEP (vertices_at sh (reachable g x) (Graph_gen_redirect_parent g' x x' H7 H8 H10))).
+    Grab Existential Variables.
+    Focus 2. {
+      simplify_ramif. apply (@graph_gen_redirect_parent_ramify _ (sSGG_VST sh)); auto.
+      apply reachable_foot_valid in H4. intro. subst x'. apply (valid_not_null g' null H4). simpl. auto.
+    } Unfocus.
+    unfold semax_ram.
+    forward. remember (Graph_gen_redirect_parent g' x x' H7 H8 H10) as g3. apply (exp_right g3).
+    apply (exp_right x'). entailer !.
+
   
 Abort.
 
